Fix untracked values; in progress Debuging the instruction addresses

x86/proofs/mlkem_keccak_f1600_loop_no_stack.ml
@@ -15,15 +15,15 @@
  (**** print_literal_from_elf "x86/mlkem/mlkem_keccak_f1600_no_stack.o";;
  ****)
 
- let GHOST_REGLIST_TAC =
+let GHOST_REGLIST_TAC =
   W(fun (asl,w) ->
         let regreads = map rator (dest_list(find_term is_list w)) in
         let regnames = map ((^) "init_" o name_of o rand) regreads in
         let ghostvars = map (C (curry mk_var) `:int64`) regnames in
         EVERY(map2 GHOST_INTRO_TAC ghostvars regreads));;
 
-let mlkem_keccak_f1600_mc_rc_bitst_2 = define_assert_from_elf
-  "mlkem_keccak_f1600_mc_rc_bitst_2" "x86/mlkem/mlkem_keccak_f1600_no_stack.o"
+let mlkem_keccak_f1600_x86_mc_2 = define_assert_from_elf
+  "mlkem_keccak_f1600_x86_mc_2" "x86/mlkem/mlkem_keccak_f1600_no_stack.o"
 [
   0x53;                    (* PUSH (% rbx) *)
   0x55;                    (* PUSH (% rbp) *)
@@ -31,9 +31,9 @@ let mlkem_keccak_f1600_mc_rc_bitst_2 = define_assert_from_elf
   0x41; 0x55;              (* PUSH (% r13) *)
   0x41; 0x56;              (* PUSH (% r14) *)
   0x41; 0x57;              (* PUSH (% r15) *)
-  0x49; 0x89; 0xf7;        (* MOV (% r15) (% rsi) *)
   0x48; 0x81; 0xec; 0xd0; 0x00; 0x00; 0x00;
                            (* SUB (% rsp) (Imm32 (word 208)) *)
+  0x49; 0x89; 0xf7;        (* MOV (% r15) (% rsi) *)
   0x48; 0xf7; 0x57; 0x08;  (* NOT (Memop Quadword (%% (rdi,8))) *)
   0x48; 0xf7; 0x57; 0x10;  (* NOT (Memop Quadword (%% (rdi,16))) *)
   0x48; 0xf7; 0x57; 0x40;  (* NOT (Memop Quadword (%% (rdi,64))) *)
@@ -514,7 +514,11 @@ let mlkem_keccak_f1600_mc_rc_bitst_2 = define_assert_from_elf
   0xc3                     (* RET *)
 ];;
 
- let MLKEM_KECCAK_F1600_EXEC_rc_bitst = X86_MK_EXEC_RULE mlkem_keccak_f1600_mc_rc_bitst_2;;
+
+let mlkem_keccak_f1600_x86_tmc_2 = define_trimmed "mlkem_keccak_f1600_x86_tmc_2" mlkem_keccak_f1600_x86_mc_2;;
+
+
+ let MLKEM_KECCAK_F1600_EXEC_2 = X86_MK_EXEC_RULE mlkem_keccak_f1600_x86_tmc_2;;
 
  let wordlist_from_memory = define
  `wordlist_from_memory(bitstate_in,0) s = [] /\
@@ -542,12 +546,12 @@ let WORDLIST_FROM_MEMORY_CONV =
 
   let MLKEM_KECCAK_F1600_SPEC = prove(
   `forall rc_pointer:int64 pc:num stackpointer:int64 bitstate_in:int64 A.
-  nonoverlapping_modulo (2 EXP 64) (pc,LENGTH mlkem_keccak_f1600_mc_rc_bitst_2) (val  stackpointer, 264) /\
-  nonoverlapping_modulo (2 EXP 64) (pc, LENGTH mlkem_keccak_f1600_mc_rc_bitst_2) (val bitstate_in,200) /\
-  nonoverlapping_modulo (2 EXP 64) (pc, LENGTH mlkem_keccak_f1600_mc_rc_bitst_2) (val rc_pointer,192) /\
+  nonoverlapping_modulo (2 EXP 64) (pc, LENGTH mlkem_keccak_f1600_x86_tmc_2) (val  stackpointer, 264) /\
+  nonoverlapping_modulo (2 EXP 64) (pc, LENGTH mlkem_keccak_f1600_x86_tmc_2) (val bitstate_in, 200) /\
+  nonoverlapping_modulo (2 EXP 64) (pc, LENGTH mlkem_keccak_f1600_x86_tmc_2) (val rc_pointer, 192) /\
 
-  nonoverlapping_modulo (2 EXP 64) (val bitstate_in,200) (val stackpointer,264) /\
   nonoverlapping_modulo (2 EXP 64) (val bitstate_in,200) (val rc_pointer,192) /\
+  nonoverlapping_modulo (2 EXP 64) (val bitstate_in,200) (val stackpointer, 264) /\
 
   nonoverlapping_modulo (2 EXP 64) (val stackpointer, 264) (val rc_pointer,192)
 
@@ -558,7 +562,7 @@ let WORDLIST_FROM_MEMORY_CONV =
   // the output of the previous interaiton will serve as an input to the following iteration
       ==> ensures x86
   // Precondition
-  (\s. bytes_loaded s (word pc) mlkem_keccak_f1600_mc_rc_bitst_2 /\
+  (\s. bytes_loaded s (word pc) mlkem_keccak_f1600_x86_tmc_2 /\
        read RIP s = word (pc + 20) /\
        read RSP s = stackpointer /\
        C_ARGUMENTS [bitstate_in; rc_pointer] s /\
@@ -576,12 +580,12 @@ let WORDLIST_FROM_MEMORY_CONV =
 
   REWRITE_TAC[SOME_FLAGS] THEN
   MAP_EVERY X_GEN_TAC [`rc_pointer:int64`; `pc:num`] THEN
-  REWRITE_TAC [(REWRITE_CONV [mlkem_keccak_f1600_mc_rc_bitst_2] THENC LENGTH_CONV) `LENGTH mlkem_keccak_f1600_mc_rc_bitst_2`] THEN
+  REWRITE_TAC [(REWRITE_CONV [mlkem_keccak_f1600_x86_tmc_2] THENC LENGTH_CONV) `LENGTH mlkem_keccak_f1600_x86_tmc_2`] THEN
 
     MAP_EVERY X_GEN_TAC [`stackpointer:int64`;`bitstate_in:int64`;`A:int64 list`] THEN
 
 
-  REWRITE_TAC[fst MLKEM_KECCAK_F1600_EXEC_rc_bitst] THEN
+  REWRITE_TAC[fst MLKEM_KECCAK_F1600_EXEC_2] THEN
   REWRITE_TAC[MAYCHANGE_REGS_AND_FLAGS_PERMITTED_BY_ABI; C_ARGUMENTS;
               ALL; ALLPAIRS; NONOVERLAPPING_CLAUSES] THEN
   DISCH_THEN(REPEAT_TCL CONJUNCTS_THEN ASSUME_TAC) THEN
@@ -600,15 +604,16 @@ let WORDLIST_FROM_MEMORY_CONV =
     ENSURES_WHILE_PAUP_TAC
     `0` (* loop_body begin number *)
     `12` (* loop_body end number *)
-    `pc + 0x60` (* loop body start PC *)
-    `pc + 0x636` (* loop backedge branch PC -- including the jmp *) 
+    `pc + 0x64` (* loop body start PC *)
+    `pc + 0x630` (* loop backedge branch PC -- including the jmp *) 
     `\i s. // loop invariant at the end of the iteration
             (read R8 s = word (2*i) /\
             read RDI s = bitstate_in /\
             read RSP s = stackpointer /\
-            read RSI s = stackpointer /\ 
+            read RSI s = stackpointer /\
             wordlist_from_memory(rc_pointer,24) s = rc_table /\
-            wordlist_from_memory(bitstate_in,25) s = MAP2 (\(x:bool) (y:(64)word). (if x then (word_not y) else y)) ([false; true;  true;  false; false; 
+            wordlist_from_memory(bitstate_in,25) s = MAP2 (\(x:bool) (y:(64)word). (if x then (word_not y) else y)) (
+              [false; false;  true;  false; false; 
               false; false; false; true;  false; 
               false; false; true;  false; false; 
               false; false; true;  false; false;
@@ -622,12 +627,26 @@ let WORDLIST_FROM_MEMORY_CONV =
           ARITH_TAC;
 
           (* program_begin until loop_entry *)
-          REWRITE_TAC[rc_table; CONS_11; GSYM CONJ_ASSOC; WORDLIST_FROM_MEMORY_CONV `wordlist_from_memory(rc_pointer,24) s:int64 list`;
-                    WORDLIST_FROM_MEMORY_CONV `wordlist_from_memory(bitstate_in,25) s:int64 list`] THEN
+
+          REWRITE_TAC[rc_table; CONS_11; GSYM CONJ_ASSOC; WORDLIST_FROM_MEMORY_CONV `wordlist_from_memory(rc_pointer,24) s:int64 list`; WORDLIST_FROM_MEMORY_CONV `wordlist_from_memory(bitstate_in,25) s:int64 list`] THEN
           ENSURES_INIT_TAC "s0" THEN
           BIGNUM_DIGITIZE_TAC "A_" `read (memory :> bytes (bitstate_in,8 * 25)) s0` THEN
-          X86_STEPS_TAC MLKEM_KECCAK_F1600_EXEC_rc_bitst (1--13) THEN
+
+          ASM_REWRITE_TAC[] THEN
+
+          (* X86_STEPS_TAC MLKEM_KECCAK_F1600_EXEC_2 (1--13) THEN *)
+
+          X86_STEPS_TAC MLKEM_KECCAK_F1600_EXEC_2 (1--1) THEN
+
+          X86_STEPS_TAC MLKEM_KECCAK_F1600_EXEC_2 (2--6) THEN
+
+            X86_STEPS_TAC MLKEM_KECCAK_F1600_EXEC_2 (7--7) THEN
+            X86_STEPS_TAC MLKEM_KECCAK_F1600_EXEC_2 (8--13) THEN
+
           ENSURES_FINAL_STATE_TAC THEN ASM_REWRITE_TAC[] THEN
+
+
+          (* In progress; Works until HERE depending on addresses in the loop invariant*)
           REPEAT CONJ_TAC THENL 
           [
                 CONV_TAC WORD_RULE;
@@ -635,33 +654,65 @@ let WORDLIST_FROM_MEMORY_CONV =
                 EXPAND_TAC "A" THEN
                 CHANGED_TAC(PURE_ONCE_REWRITE_TAC[ARITH_RULE `2 * 0 = 0`]) THEN
 
-                CHANGED_TAC(REWRITE_TAC[keccak; MAP2]);
+                CHANGED_TAC(REWRITE_TAC[keccak]) THEN 
+                CHANGED_TAC(REWRITE_TAC[MAP2;CONS_11]);
           ]
+
           REPEAT STRIP_TAC THEN
 
-          REWRITE_TAC[rc_table; CONS_11; GSYM CONJ_ASSOC; WORDLIST_FROM_MEMORY_CONV `wordlist_from_memory(rc_pointer,24) s:int64 list`;
-                    WORDLIST_FROM_MEMORY_CONV `wordlist_from_memory(bitstate_in,25) s:int64 list`] THEN
+          GHOST_INTRO_TAC `init_rax:int64` `read RAX` THEN
+          GHOST_INTRO_TAC `init_rbx:int64` `read RBX` THEN
+          GHOST_INTRO_TAC `init_rcx:int64` `read RCX` THEN
+          GHOST_INTRO_TAC `init_rdx:int64` `read RDX` THEN
+          GHOST_INTRO_TAC `init_rbp:int64` `read RBP` THEN
+          GHOST_INTRO_TAC `init_r8:int64` `read R8` THEN
+          GHOST_INTRO_TAC `init_r15:int64` `read R15` THEN
+
+          
+
+          REWRITE_TAC[rc_table; CONS_11; GSYM CONJ_ASSOC; WORDLIST_FROM_MEMORY_CONV `wordlist_from_memory(rc_pointer,24) s:int64 list`; WORDLIST_FROM_MEMORY_CONV `wordlist_from_memory(bitstate_in,25) s:int64 list`] THEN
           ENSURES_INIT_TAC "s0" THEN
-          BIGNUM_DIGITIZE_TAC "A'_" `read (memory :> bytes (bitstate_in,8 * 25)) s0` THEN
+          BIGNUM_DIGITIZE_TAC "A_" `read (memory :> bytes (bitstate_in,8 * 25)) s0` THEN 
+          
+          ASM_REWRITE_TAC[] THEN
 
-          (*non overlapping!!*)
-           X86_STEPS_TAC MLKEM_KECCAK_F1600_EXEC_rc_bitst (1--1) THEN
-           X86_STEPS_TAC MLKEM_KECCAK_F1600_EXEC_rc_bitst (2--5) THEN
+                X86_STEPS_TAC MLKEM_KECCAK_F1600_EXEC_2 (1--1) THEN
+                X86_STEPS_TAC MLKEM_KECCAK_F1600_EXEC_2 (2--5) THEN
 
-           X86_STEPS_TAC MLKEM_KECCAK_F1600_EXEC_rc_bitst (6--395) THEN
 
-            ENSURES_FINAL_STATE_TAC THEN ASM_REWRITE_TAC[] THEN
+                 X86_STEPS_TAC MLKEM_KECCAK_F1600_EXEC_2 (6--6) THEN
+                 X86_STEPS_TAC MLKEM_KECCAK_F1600_EXEC_2 (7--10) THEN
+
+                 X86_STEPS_TAC MLKEM_KECCAK_F1600_EXEC_2 (11--390) THEN
+
+              
+
+                  X86_STEPS_TAC MLKEM_KECCAK_F1600_EXEC_2 (391--394) THEN
+
+
+
+          ENSURES_FINAL_STATE_TAC THEN ASM_REWRITE_TAC[] THEN
+          
             REPEAT CONJ_TAC THENL [
               (* r 1 ;; *)
                CONV_TAC WORD_RULE;
+
+               SUBST1_TAC(MESON[MULT_CLAUSES] `keccak 2 = keccak (2 * 1)`) THEN
+
+               PURE_ONCE_REWRITE_TAC[ARITH_RULE `2 * 1 = (0 + 1) + 1`] THEN 
 
 
                 EXPAND_TAC "A" THEN
 
                 CHANGED_TAC(PURE_ONCE_REWRITE_TAC[ARITH_RULE `2 * (i + 1) = (2 * i + 2)`]) THEN
+
+                CHANGED_TAC(PURE_ONCE_REWRITE_TAC[ARITH_RULE `2 = (0 + 1) + 1`]) THEN
+
                  CONV_TAC WORD_RULE THEN
 
                  ASM_REWRITE_TAC[] THEN
+
+                 GEN_REWRITE_TAC THEN
 
 
                 CHANGED_TAC(PURE_ONCE_REWRITE_TAC[ARITH_RULE `2 * i + 2 = (2 * i + ((0 + 1) + 1))`]) THEN
@@ -710,7 +761,7 @@ CONV_TAC(ONCE_DEPTH_CONV EL_CONV) THEN
     
 REPEAT CONJ_TAC THEN BITBLAST_TAC; *)
 
-      (* X86_SIM_TAC MLKEM_KECCAK_F1600_EXEC_rc_bitst (1--21); *)
+      (* X86_SIM_TAC MLKEM_KECCAK_F1600_EXEC_2 (1--21); *)
 
       (* the body of the loop *)
      
@@ -720,7 +771,7 @@ REPEAT CONJ_TAC THEN BITBLAST_TAC; *)
       REPEAT CONJ_TAC THENL
       REWRITE_TAC[rc_table; CONS_11; GSYM CONJ_ASSOC; WORDLIST_FROM_MEMORY_CONV `wordlist_from_memory(rc_pointer,24) s:int64 list`] THEN
 
-     X86_SIM_TAC MLKEM_KECCAK_F1600_EXEC_rc_bitst (1--394) THEN
+     X86_SIM_TAC MLKEM_KECCAK_F1600_EXEC_2 (1--394) THEN
 
       REPEAT CONJ_TAC THENL
       [
@@ -748,12 +799,12 @@ REPEAT CONJ_TAC THEN BITBLAST_TAC; *)
 
       (* Prove that backedge is taken if i != 12. *)
       REPEAT STRIP_TAC THEN
-      X86_SIM_TAC MLKEM_KECCAK_F1600_EXEC_rc_bitst [1];
+      X86_SIM_TAC MLKEM_KECCAK_F1600_EXEC_2 [1];
 
        REWRITE_TAC[condition_semantics] THEN REPEAT CONJ_TAC THENL
       REWRITE_TAC[rc_table; CONS_11; GSYM CONJ_ASSOC; WORDLIST_FROM_MEMORY_CONV `wordlist_from_memory(rc_pointer,24) s:int64 list`] THEN
       
 
       (* Loop exit to the end of the program *)
-      X86_SIM_TAC MLKEM_KECCAK_F1600_EXEC_rc_bitst (1--16);
+      X86_SIM_TAC MLKEM_KECCAK_F1600_EXEC_2 (1--16);
   ]);
